\documentclass{article}
\title{Homework 7}
\author{Zachary Moring}

\usepackage{amsmath,amssymb}
\usepackage{boxproof}
\usepackage{hyperref}
\usepackage{tikz}
\usepackage{forest}

\newcommand{\Hide}[1]{}
\newcommand{\code}[1]{\texttt{#1}}
\newcommand{\Intro}[1]{{#1}{\textrm{i}}}
\newcommand{\Elim}[1]{{#1}{\textrm{e}}}
\newcommand{\Premise}{\textrm{premise}}
\newcommand{\Let}{\textrm{let}}
\newcommand{\Assume}{\textrm{assume}}
\newcommand{\Break}{\vspace{0.2cm}\hrule{}\vspace{0.2cm}}
\newcommand{\tIf}{\text{if }}
\newcommand{\all}{\forall}

\begin{document} \maketitle

Code for this assignment is at:
\url{https://github.com/zpm-bu/cs511-formal-methods/blob/assignments/lean/Homework/hw7.lean}

\newpage{}

\vspace{1in}

\noindent\textbf{Exercise 1.} Use first-order ground tableaux to show that
$\Gamma \vDash \varphi$ where
\[
  \Gamma \overset{\text{def}}{=} \left\{ \forall x \forall y \forall z
  \left( P(x, y) \wedge P(y, z) \to P(x, z) \right), \forall x \forall y
  \left( P(x, y) \to P(y, x) \right) \right\}
\]
and
\[
  \varphi \overset{\text{def}}{=} \forall x \forall y \forall z \left(
  P(x, y) \wedge P(z, y) \to P(x, z) \right)
\]
and $P$ is an arbitrary binary predicate.

\Break{}

\scalebox{0.7}{
  \begin{forest}
    [$\Gamma \cup \{ \varphi \}$
    [{$\forall x \forall y \forall z (P(x, y) \wedge P(y, z) \to P(x, z))$}
    [{$\forall y \forall z (P(t, y) \wedge P(y, z) \to P(t, z))$}
    [{$\forall z (P(t, u) \wedge P(u, z) \to P(t, z))$}
    [{$P(t, u) \wedge P(u, v) \to P(t, v)$}
    [{$\lnot \forall x \forall y \forall z (P(x, y) \wedge P(z, y) \to P(x, z))$}
    [{$\lnot \forall y \forall z (P(t, y) \wedge P(z, y) \to P(t, z))$}
    [{$\lnot \forall z P(t, u) \wedge P(z, u) \to P(t, z)$}
    [{$\lnot (P(t, u) \wedge P(v, u) \to P(t, v))$}
    [{$P(t, u) \wedge P(v, u)$}
    [{$\lnot P(t, v)$}
    [{$P(t, u)$}
    [{$P(v, u)$}
    [{$\forall x \forall y P(x, y) \to P(y, x)$}
    [{$\forall y P(v, y) \to P(y, v)$}
    [{$P(v, u) \to P(u, v)$}
    [{$\lnot (P(t, u) \wedge P(u, v))$}
    [{$\lnot P(t, u)$}\\{$\times$} ]
    [{$\lnot P(u, v)$}
    [{$\lnot P(v, u)$}\\{$\times$} ]
    [{$P(u, v)$}\\{$\times$} ]
    ]
    ]
    [{$P(t, v)$}\\{$\times$} ]
    ] ] ] ] ] ] ] ] ] ] ] ] ] ] ] ]
  \end{forest}
}

\newpage{}

\noindent\textbf{Exercise 2.} Use first-order ground tableaux to show...

\Break{}

\scalebox{0.7}{
  \begin{forest}
    [$\Gamma \cup \{ \varphi \}$
    [{$\forall x Q(x, a, a)$}
    [{$Q(a, s^2(a), s^2(a))$}
    [{$\forall x \forall y \forall z (Q(x, y, z) \to Q(x, s(y), s(z)))$}
    [{$\forall x \forall y \forall z (Q(x, y, z) \to Q(y, x, z))$}
    [{$\lnot \exists x Q(s^2(a), s^3(a), x)$}
    [{$\lnot Q(s^2(a), s^3(a), s^5(a))$}
    [{$\forall y \forall z ( Q(a, y, z) \to Q(y, a, z) )$}
    [{$\forall z (Q(a, s^2(a), z) \to Q(s^2(a), a, z))$}
    [{$Q(a, s^2(a), s^2(a)) \to Q(s^2(a), a, s^2(a))$}
    [{$\forall y \forall z Q(s^2(a), y, z) \to Q(s^2(a), s(y), s(z))$}
    [{$\forall z Q(s^2(a), a, z) \to q(s^2(a), s(a), s(z))$}
    [{$Q(s^2(a), a, s^2(a)) \to Q(s^2(a), s(a), s^3(a))$}
    [{$Q(s^2(a), s(a), s^3(a)) \to Q(s^2(a), s^2(a), s^4(a))$}
    [{$Q(s^2(a), s^2(a), s^4(a)) \to Q(s^2(a), s^3(a), s^5(a))$}
      [{$\lnot Q(a, s^2(a), s^2(a)) \times$} ]
      [{$Q(s^2(a), a, s^2(a))$}
        [{$\lnot Q(s^2(a), a, s^2(a)) \times$} ]
        [{$Q(s^2(a), s(a), s^3(a))$}
          [{$\lnot Q(s^2(a), s(a), s^3(a)) \times$} ]
          [{$Q(s^2(a), s^2(a), s^4(a))$}
            [{$\lnot Q(s^2(a), s^2(a), s^4(a)) \times$} ]
            [{$Q(s^2(a), s^3(a), s^5(a)) \times$} ]
          ]
        ]
      ]
    ] ] ] ] ] ] ] ] ] ] ] ] ] ] ]
  \end{forest}
}

\end{document}
